extraction/Extr.v
@@ -1,4 +1,7 @@
 From Stdlib Require Import Extraction.
-From Rocqeteer Require Import EffIR.
+From Rocqeteer Require Import EffIR Samples.
 Extraction Language OCaml.
-Separate Extraction EffIR.prog0 EffIR.observe.
+Separate Extraction
+  EffIR.prog0 EffIR.observe EffIR.run
+  Samples.sample_delete Samples.sample_two Samples.sample_ret
+  Samples.sample_neg Samples.sample_nested.
